LeanProjeto2/StarLanguage/ResultsAndOtherDefinitions.lean
@@ -2,14 +2,22 @@
 --       STAR LANGUAGE - RESULTS and OTHER DEFINITIONS
 -- -------------------------------------------------------------
 
--- We import the definitions from the first-order language L:
 import LeanProjeto2.FOLanguage
-import LeanProjeto2.StarLanguage.FiniteTypes
-import LeanProjeto2.StarLanguage.Syntax
 import LeanProjeto2.StarLanguage.Axioms2
+import LeanProjeto2.StarLanguage.Syntax
+import LeanProjeto2.StarLanguage.FiniteTypes
 import MathLib.Tactic
+import Mathlib.Data.Finset.Basic
+import Mathlib.Data.Multiset.Basic
+import Batteries
 
+open LFormula
+open Term
+open Formula
+open Set
+open Batteries
 
+/-
 #check 5
 #check 5+3
 
@@ -25,3 +33,4 @@ lemma AddResult (m n l : ℕ) : m+(n+l) = l+(n+m) :=
 lemma AddResult2 (m n l : ℕ) : m+(n+l) = l+(n+m) :=
   by
     linarith
+-/
